\begin{CajaTitulo}{\begin{center}\subsection{Solución P7}\end{center}}
    \vspace{0.7cm}

    \[\int_{0}^{\infty}e^{-x^2}\cos(x)dx \implies \int_{0}^{\infty}e^{-x^2}\cos(ax)dx \:=\: \I(a) , \hspace{0.3cm}I(0) = \frac{\sqrt{\pi}}{2} \]
    \[\frac{d}{da}\int_{0}^{\infty}e^{-x^2}\cos(ax)dx \:= \: \I'(a) \implies \int_{0}^{\infty}\frac{\partial}{\partial a}e^{-x^2}\cos(ax)dx  = \int_{0}^{\infty}e^{-x^2}\sin(ax)(-x)dx\]
    \\
    Integrando por partes, obtenemos que:
    \[\PorPartes{\sin(ax)}{\cos(ax) \cdot (a) dx}{e^{-x^2}(-x)dx}{\frac{e^{-x^2}}{2}} =   \frac{e^{-x^2}}{2} \sin(ax) \Brackets_{0}^{\infty}  - \frac{a}{2}\int_{0}^{\infty}e^{-x^2}\cos(ax)dx     \]
    \[\I'(a) = - \frac{a}{2}\int_{0}^{\infty}e^{-x^2}\cos(ax)dx = - \frac{a}{2}\I(a), \hspace{1cm} \Porlo \hspace{0.2cm} \frac{\I'(a)}{\I(a)} = \frac{-a}{2}  \]
    \[\int \frac{\I'(a)}{\I(a)}da = \int \frac{-a}{2} da \implies \ln(\I(a)) = \frac{-a^2}{4} + C, \: \: \I(a) = e^{\frac{-a^2}{4} + C}\]

    Para $\I(0)$, tenemos que: $\I(0) = e^{\frac{-0^2}{4} + C} = e^{C} = \frac{\sqrt{\pi}}{2} \implies C = \ln(\mathlarger{\frac{\sqrt{\pi}}{2}})$ Entonces, $\I(a) = e^{\frac{-a^2}{4} + \ln(\frac{\sqrt{\pi}}{2})} = \mathlarger{ \frac{\sqrt{\pi}}{2}e^{\mathlarger{\frac{-a^2}{4}}}}$

    \[\I(a) = \int_{0}^{\infty}e^{-x^2}\cos(ax)dx = \frac{\sqrt{\pi}}{2}e^{\mathlarger{\frac{-a^2}{4}}}\]
    \[\I(1) = \int_{0}^{\infty}e^{-x^2}\cos(x)dx =  \frac{\sqrt{\pi}}{2}e^{\mathlarger{\frac{-1}{4}}}  \hspace{1cm}\square\]

    Demostración de la integral de Gaussiana:
    \\

    Consideremos la siguiente función:

    \[\I(a) = \int_{0}^{\infty}\frac{ e^{-a^2(1+x^2)}}{1 + x^2}dx \hspace{0.2cm} \Flecha{\mathlarger{\frac{d}{da}}} \: \: \I'(a) = \int_{0}^{\infty}e^{-a^2(1+x^2)}(-2a) = (-2a)e^{-a^2}\int_{0}^{\infty}e^{-(ax)^2} dx \]
    \[\I'(a) = (-2a)e^{-a^2} \int_{0}^{\infty}e^{-{(ax)}^2} dx \hspace{0.2cm}   \cambio{ax = u}{dx \cdot a = du} = (-2) e^{-a^2} \int_{0}^{\infty}e^{-{u}^2}du\]
    \[\int_{0}^{\infty}\I'(a)da = (-2) \int_{0}^{\infty}e^{-a^2}da \int_{0}^{\infty}e^{-{u}^2}du \implies \I(\infty) - \I(0) = -2 \left(\int_{0}^{\infty}e^{-{u}^2}du\right)^2\]
    \[\frac{-\pi}{2} = -2\left(\int_{0}^{\infty}e^{-{u}^2}du\right)^2 \hspace{0.2cm}\]
    \[ \Porlo  \int_{0}^{\infty}e^{-x^2}dx = \frac{\sqrt{\pi}}{2}\]
\end{CajaTitulo}